modified the program semantic
an alligned jump in the header leads to an alligned jump anywhere in the code

a non alligned jump in the header lead to a DANGER_STATE

NTCB/Semantics.v
@@ -1,6 +1,7 @@
 Require Import Lib.
 Require Import BinaryProps.
 Require Import List.
+Require Import Program.
 
 Set Implicit Arguments.
 (* move to lib *)
@@ -244,14 +245,99 @@ Module Type INSTRUCTION_SEMANTICS(Import I: INSTRUCTION).
 
 End INSTRUCTION_SEMANTICS.
 
+Fixpoint pow2 (n: nat) :=
+  match n with
+    | O => 1
+    | S n' => 2 * pow2 n'
+  end.
+
+
+Definition dividable_by_pow2 (p: nat) (n:N) :=
+  exists d:N, n = (pow2 p) * d.
+
+Lemma dividable_by_pow2_dec:
+  forall p n, {dividable_by_pow2 p n}+{~dividable_by_pow2 p n}.
+Proof.
+  unfold dividable_by_pow2.
+  intros. destruct' n as [|pos].
+  Case "0".
+  left. exists 0. zify. omega.
+  Case "Npos pos".
+  revert p.
+  induction' pos as [pos|pos|]; intros.
+  SCase "xI pos".
+  destruct' p as [|p'].
+    SSCase "0%nat".
+    left. exists (Npos pos~1). reflexivity.
+    SSCase "S p'".
+    right. intros [d H]. simpl in H. destruct (pow2 p').
+      inv H.
+      simpl in H. destruct d; inv H.
+
+   SCase "xO pos".
+   destruct' p as [|p'].
+   SSCase "0%nat".
+     left. exists (Npos pos~0). reflexivity.
+   SSCase "S p'".
+     destruct' (IHpos p') as [EXISTS|NEXISTS].
+     S3Case "left EXISTS".
+       left. destruct EXISTS as [d H].
+       exists d. simpl. destruct (pow2 p'). inv H.
+       simpl. destruct d. inv H. inv H. reflexivity.
+
+     S3Case "right NEXISTS".
+       right. intros [d H].
+       apply NEXISTS.
+       simpl in H. destruct (pow2 p'). inv H.
+       exists d. simpl. destruct d; inv H. reflexivity.
+
+  SCase "1%positive".
+   destruct' p as [|p'].
+   SSCase "0%nat".
+     left. exists 1. reflexivity.
+   SSCase "S p'".
+     right. intros [d H]. simpl in H. destruct (pow2 p'); inv H.
+     destruct d; inv H1.
+Qed.
+
+Definition dividable_by_32 (n:N) :=
+  exists d:N, n = 32 * d.
+
+Program Definition dividable_by_32_dec n
+  : {dividable_by_32 n} + {~dividable_by_32 n}:=
+  match n with
+    | N0 => left _
+    | Npos p~0~0~0~0~0 => left _
+    | Npos _ => right _
+  end.
+Next Obligation.
+  unfold dividable_by_32. exists 0. reflexivity.
+Qed.
+Next Obligation.
+  unfold dividable_by_32. simpl. exists (Npos p). reflexivity.
+Qed.
+Next Obligation.
+  destruct wildcard' as [wildcard'|wildcard'|]; try solve
+    [let H0 := fresh "H" in intros [[|?] H0]; simpl in H0; inv H0].
+  destruct wildcard' as [wildcard'|wildcard'|]; try solve
+    [let H0 := fresh "H" in intros [[|?] H0]; simpl in H0; inv H0].
+  destruct wildcard' as [wildcard'|wildcard'|]; try solve
+    [let H0 := fresh "H" in intros [[|?] H0]; simpl in H0; inv H0].
+  destruct wildcard' as [wildcard'|wildcard'|]; try solve
+    [let H0 := fresh "H" in intros [[|?] H0]; simpl in H0; inv H0].
+  destruct wildcard' as [wildcard'|wildcard'|]; try solve
+    [let H0 := fresh "H" in intros [[|?] H0]; simpl in H0; inv H0].
+  intro. apply (H wildcard'). reflexivity.
+Qed.
+
+
+
 (* Define the semantics of programs, parameterized by those of instruction *)
 Module Prog_Semantics (Import I: INSTRUCTION)(Import IS:INSTRUCTION_SEMANTICS(I)).
 
   Inductive target_state :=
     (* a regular state *)
   | Normal_state: state register -> target_state
-    (* after a jump in the header *)
-  | Header_code : state register -> target_state
     (* after a jump outside of the code segment *)
   | Non_executable_code: state register -> target_state
     (* a state that should *never* be reached ! *)
@@ -277,11 +363,29 @@ Module Prog_Semantics (Import I: INSTRUCTION)(Import IS:INSTRUCTION_SEMANTICS(I)
     read_instr_from_memory st1.(state_mem) st1.(state_pc) = Some (instr, n) ->
     instruction_semantics (header_size + code_size) instr st1 Bad_state ->
     step header_size code_size st1 DANGER_STATE
-  | Step_header: forall instr n st2,
+
+    (* if we jump in the header, it must be at a correct address *)
+  | Step_header_bad: forall instr n st2,
     read_instr_from_memory st1.(state_mem) st1.(state_pc) = Some (instr, n) ->
     instruction_semantics (header_size + code_size) instr st1 (Good_state st2) ->
-    st2.(state_pc) < header_size ->
-    step header_size code_size st1 (Header_code st2)
+    st2.(state_pc) < header_size -> ~dividable_by_32 st2.(state_pc) ->
+    step header_size code_size st1 DANGER_STATE
+
+    (* if the address in the header is correct, we can jump anywhere in the code *)
+
+  | Step_header_good: forall instr n st2,
+    read_instr_from_memory st1.(state_mem) st1.(state_pc) = Some (instr, n) ->
+    instruction_semantics (header_size + code_size) instr st1 (Good_state st2) ->
+    st2.(state_pc) < header_size -> dividable_by_32 st2.(state_pc) ->
+    forall m2 regs2 pc2,
+      same_code (header_size + code_size) st2.(state_mem) m2 ->
+      header_size <= pc2 -> pc2 < header_size + code_size ->
+      dividable_by_32 pc2 ->
+      step header_size code_size st1
+        (Normal_state {| state_mem := m2;
+                         state_pc := pc2;
+                         state_regs := regs2 |})
+
   | Step_outside: forall instr n st2,
     read_instr_from_memory st1.(state_mem) st1.(state_pc) = Some (instr, n) ->
     instruction_semantics (header_size + code_size) instr st1 (Good_state st2) ->
@@ -295,8 +399,18 @@ Module Prog_Semantics (Import I: INSTRUCTION)(Import IS:INSTRUCTION_SEMANTICS(I)
        segment because of multi threading *)
     forall m2', same_code (header_size + code_size) m2' st2.(state_mem) ->
     step header_size code_size st1
-      (Normal_state {| state_mem := m2'; state_pc := st2.(state_pc); state_regs :=st2.(state_regs) |}).
+      (Normal_state {| state_mem := m2';
+                       state_pc := st2.(state_pc);
+                       state_regs :=st2.(state_regs) |}).
 
+
+  Inductive accessible_state (header_size code_size: N)
+    (st1: state register): state register -> Prop :=
+  | AS0: accessible_state header_size code_size st1 st1
+  | ASS: forall st2 st3,
+    step header_size code_size st1 (Normal_state st2) ->
+    accessible_state header_size code_size st2 st3 ->
+    accessible_state header_size code_size st1 st3.
 
   (* is DANGER_STATE accessible from a state ? *)
   Inductive accessible_danger (header_size code_size: N) (st1: state register) : Prop :=
